Birthday refinements
Allows prameterised sampling and bounding of collisions up to a function
The query bound is now provided as a lemma parameter unless the oracles enforce the query bound.

theories/crypto/Birthday.ec
@@ -4,28 +4,34 @@ require import StdRing StdOrder StdBigop FelTactic.
 require (*--*) Mu_mem.
 (*---*) import RField IntOrder RealOrder.
 
-(** A non-negative integer q **)
-op q : { int | 0 <= q } as ge0_q.
+(** An input type **)
+type in_t.
 
-(** A type T equipped with its full uniform distribution **)
-type T.
+(** An output type out_t with an input-parameterised distribution **)
+type out_t.
 
-op uT: T distr.
-op maxu : T.
-axiom maxuP x: mu1 uT x <= mu1 uT maxu.
+op dout: in_t -> out_t distr.
 
-(** A module that samples in uT on queries to s **)
+(**
+(** A further transformation under which we catch collisions **)
+type fin_t.
+
+op f : out_t -> fin_t.
+op pr_predict : { real | forall x y, mu1 (dmap (dout x) f) y <= pr_predict }
+  as predictP.
+**)
+(** A module that samples in `dout x` on queries `s(x)` **)
 module Sample = {
-  var l:T list
+  var l : out_t list
 
   proc init(): unit = {
     l <- [];
   }
 
-  proc s(): T = {
+  proc s(x : in_t): out_t = {
     var r;
 
-    r <$ uT;
+    r <$ dout x;
     l <- r::l;
     return r;
   }
@@ -33,25 +39,23 @@ module Sample = {
 
 module type Sampler = {
   proc init(): unit
-  proc s(): T
+  proc s(_ : in_t): out_t
 }.
 
 (** Adversaries that may query an s oracle **)
 module type ASampler = {
-  proc s(): T
+  include Sampler [s]
 }.
 
-module type Adv(S:ASampler) = {
+module type Adv (S : ASampler) = {
   proc a(): unit
 }.
 
 (** And an experiment that initializes the sampler and runs the adversary **)
-module Exp(S:Sampler,A:Adv) = {
-  module A = A(S)
-
+module Exp (S : Sampler) (A : Adv) = {
   proc main(): unit = {
     S.init();
-    A.a();
+    A(S).a();
   }
 }.
 
@@ -62,85 +66,98 @@ section.
   declare module A <: Adv {-Sample}.
   declare axiom A_ll (S <: ASampler {-A}): islossless S.s => islossless A(S).a.
 
+  declare op q : { int | 0 <= q } as ge0_q.
+
+  declare type fin_t.
+  declare op f : out_t -> fin_t.
+
+  declare op pr_predict : { real | forall x y, mu1 (dmap (dout x) f) y <= pr_predict }
+    as predictP.
+
   lemma pr_Sample_le &m:
-    Pr[Exp(Sample,A).main() @ &m : size Sample.l <= q /\ !uniq Sample.l]
-    <= (q*(q-1))%r/2%r * mu1 uT maxu.
+       Pr[Exp(Sample,A).main() @ &m : size Sample.l <= q /\ !uniq (map f Sample.l)]
+    <= (q * (q - 1))%r/2%r * pr_predict.
   proof.
-    fel 1 (size Sample.l) (fun x, x%r * mu1 uT maxu) q (!uniq Sample.l) []=> //.
-    + by rewrite -Bigreal.BRA.mulr_suml  Bigreal.sumidE 1:ge0_q.
-    + by inline*; auto.
-    + proc;wp; rnd (mem Sample.l); skip=> // /> &hr ???.
-      apply (Mu_mem.mu_mem_le_size (Sample.l{hr}) uT (mu1 uT maxu)). 
-      by move=> x _;rewrite maxuP.
-    by move=> c; proc; auto=> /#.
+  fel 1 (size Sample.l) (fun x, x%r * pr_predict) q (!uniq (map f Sample.l)) []=> //.
+  + by rewrite -Bigreal.BRA.mulr_suml  Bigreal.sumidE 1:ge0_q.
+  + by inline*; auto.
+  + proc;wp; rnd (mem (map f Sample.l) \o f); skip=> // /> &hr ???.
+    rewrite -dmapE -(size_map f).
+    apply: (Mu_mem.mu_mem_le_size (map f Sample.l{hr}) (dmap (dout x{hr}) f) pr_predict). 
+    by move=> x _;rewrite predictP.
+  by move=> c; proc; auto=> /#.
   qed.
 
   lemma pr_Sample_le_q2 &m:
-    Pr[Exp(Sample,A).main() @ &m: size Sample.l <= q /\ !uniq Sample.l]
-    <= (q^2)%r * mu1 uT maxu.
+    Pr[Exp(Sample,A).main() @ &m: size Sample.l <= q /\ !uniq (map f Sample.l)]
+    <= (q^2)%r * pr_predict.
   proof.
-    apply (ler_trans _ _ _ (pr_Sample_le &m)). 
-    apply ler_wpmul2r; 1: by apply ge0_mu. 
-    have -> : q^2 = q*q by ring.
-    smt(ge0_q).
+  apply (ler_trans _ _ _ (pr_Sample_le &m)). 
+  apply ler_wpmul2r.
+  + exact/(ler_trans _ _ _ _ (predictP witness witness))/ge0_mu.
+  have -> : q^2 = q*q by ring.
+  smt(ge0_q).
   qed.
 
   declare axiom A_bounded: hoare [A(Sample).a : size Sample.l = 0 ==> size Sample.l <= q].
 
-  local lemma aux &m : 
-    Pr[Exp(Sample,A).main() @ &m: !uniq Sample.l] =
-    Pr[Exp(Sample,A).main() @ &m: size Sample.l <= q /\ !uniq Sample.l].
+  local lemma aux &m :
+      Pr[Exp(Sample,A).main() @ &m: !uniq (map f Sample.l)]
+    = Pr[Exp(Sample,A).main() @ &m: size Sample.l <= q /\ !uniq (map f Sample.l)].
   proof.
-    byequiv (_: ={glob A} ==> ={Sample.l} /\ size Sample.l{2} <= q)=> //=.
-    conseq (_: _ ==> ={Sample.l}) _ (_: _ ==> size Sample.l <= q)=> //=;2:by sim.
-    by proc;call A_bounded;inline *;auto.
+  byequiv (: ={glob A} ==> ={Sample.l} /\ size Sample.l{2} <= q)=> //=.
+  conseq (: _ ==> ={Sample.l}) _ (: _ ==> size Sample.l <= q)=> //=;2:by sim.
+  by proc; call A_bounded; inline *; auto.
   qed.
 
   lemma pr_collision &m:
-    Pr[Exp(Sample,A).main() @ &m: !uniq Sample.l]
-    <= (q*(q-1))%r/2%r* mu1 uT maxu.
-  proof. rewrite (aux &m); apply (pr_Sample_le &m). qed.
+       Pr[Exp(Sample,A).main() @ &m: !uniq (map f Sample.l)]
+    <= (q * (q - 1))%r / 2%r * pr_predict.
+  proof. by rewrite (aux &m); exact: (pr_Sample_le &m). qed.
 
   lemma pr_collision_q2 &m:
-    Pr[Exp(Sample,A).main() @ &m: !uniq Sample.l]
-    <= (q^2)%r * mu1 uT maxu.
-  proof. rewrite (aux &m); apply (pr_Sample_le_q2 &m). qed.
+       Pr[Exp(Sample,A).main() @ &m: !uniq (map f Sample.l)]
+    <= (q^2)%r * pr_predict.
+  proof. by rewrite (aux &m); apply (pr_Sample_le_q2 &m). qed.
 
 end section.
 
 (*** The same result using a bounding module ***)
-module Bounder(S:Sampler) = {
-  var c:int
+abstract theory BoundedOracle.
+op q : { int | 0 <= q } as ge0_q.
+
+module Bounder (S : Sampler) = {
+  var c : int
 
   proc init(): unit = {
-    S.init();
+         S.init();
     c <- 0;
   }
 
-  proc s(): T = {
+  proc s(x : in_t): out_t = {
     var r <- witness;
 
     if (c < q) {
-      r <@ S.s();
+      r <@ S.s(x);
       c <- c + 1;
     }
     return r;
   }
 }.
 
-module ABounder(S:ASampler) = {
-  proc s(): T = {
+module ABounder (S : ASampler) = {
+  proc s(x : in_t): out_t = {
     var r <- witness;
 
     if (Bounder.c < q) {
-      r         <@ S.s();
+      r         <@ S.s(x);
       Bounder.c <- Bounder.c + 1;
     }
     return r;
   }
 }.
 
-module Bounded(A:Adv,S:ASampler) = {
+module Bounded (A : Adv) (S : ASampler) = {
   proc a(): unit = {
     Bounder.c <- 0;
     A(ABounder(S)).a();
@@ -149,31 +166,37 @@ module Bounded(A:Adv,S:ASampler) = {
 
 equiv PushBound (S <: Sampler {-Bounder}) (A <: Adv {-S,-Bounder}):
   Exp(Bounder(S),A).main ~ Exp(S,Bounded(A)).main:
-    ={glob A,glob S} ==>
-    ={glob A,glob S}.
-proof. by proc; inline*; sim. qed.
+    ={glob A, glob S} ==> ={glob A,glob S}.
+proof. by proc; inline *; sim. qed.
 
 (** Forall adversary A with access to the bounded s oracle, the
     probability that the same output is sampled twice is bounded by
     q^2/|T|                                                         **)
 section.
-  declare module A <: Adv {-Sample,-Bounder}.
-
+  declare module A <: Adv {-Sample, -Bounder}.
   declare axiom A_ll (S <: ASampler {-A}): islossless S.s => islossless A(S).a.
 
+  declare type fin_t.
+  declare op f : out_t -> fin_t.
+
+  declare op pr_predict : { real | forall x y, mu1 (dmap (dout x) f) y <= pr_predict }
+    as predictP.
+
+
   lemma pr_collision_bounded_oracles &m:
-    Pr[Exp(Bounder(Sample),A).main() @ &m: !uniq Sample.l]
-    <= (q^2)%r * mu1 uT maxu.
+       Pr[Exp(Bounder(Sample),A).main() @ &m: !uniq (map f Sample.l)]
+    <= (q^2)%r * pr_predict.
   proof.
-    have ->: Pr[Exp(Bounder(Sample),A).main() @ &m: !uniq Sample.l] =
-             Pr[Exp(Sample,Bounded(A)).main() @ &m: !uniq Sample.l].
-    + byequiv (PushBound Sample A) => //.
-    apply (pr_collision_q2 (Bounded(A)) _ _ &m).
-    + move=> S HS;proc;call (A_ll (ABounder(S)) _);2:by auto.
-      by proc;sp;if;auto;call HS.     
-    proc; call (_: size Sample.l <= Bounder.c <= q).
-    + proc;sp;if=>//;inline *;auto=> /#.
-    auto;smt w=ge0_q.
+  have ->: Pr[Exp(Bounder(Sample),A).main() @ &m: !uniq (map f Sample.l)] =
+           Pr[Exp(Sample,Bounded(A)).main() @ &m: !uniq (map f Sample.l)].
+  + by byequiv (PushBound Sample A).
+  apply (pr_collision_q2 (Bounded(A)) _ _ ge0_q _ _ predictP _ &m)=> //.
+  + move=> S HS; proc; call (A_ll (ABounder(S)) _); 2:by auto.
+    by proc; sp; if; auto; call HS.
+  move=> /=; proc; call (: size Sample.l <= Bounder.c <= q).
+  + by proc; sp; if=> //; inline *; auto=> /#.
+  by auto; smt(ge0_q).
   qed.
 
 end section.
+end BoundedOracle.
